new/generatedproof/github_com/goose_lang/goose/testdata/examples/unittest.v
@@ -2830,4 +2830,9 @@ Global Instance wp_method_call_S'ptr_writeB :
   ltac:(apply wp_method_call'; reflexivity).
 
 End names.
+
+Global Instance wp_globals_alloc_inst `{!heapGS Σ} `{!goGlobalsGS Σ} :
+  WpGlobalsAlloc unittest.vars' (GlobalAddrs) (@var_addrs) (λ (_: GlobalAddrs), own_allocated).
+Proof. solve_wp_globals_alloc. Qed.
+
 End unittest.
